%%%%%%%%%%%%%%%%%% ANOTHER LECTURE

\chapter{Cartan Calculations in (semi)Riemannian Geometry}

Before continuing, a change of notation will be made. Although this can be confusing, the previous notation is used often by mathematicians, while the following is used by physicist.

\section{Frame Fields in (semi)Riemannian Geometry}

%Before continuing, a change of notation will be made. Although this can be confusing, the previous notation is used often by mathematicians, while the following is used by physicist.

Let $M$ be a manifold, and $g$ a (semi)Riemannian metric defined on $M$. Then the line element for the metric $g$ is
\begin{align}
  \de{s}^2(g) = g_{\mu\nu} \de{x}^\mu \otimes \de{x}^\nu.
\end{align}
Nonetheless, the information about the metric structure of the manifold can be translate to the languages of frames,
\begin{equation}
  \begin{split}
    \de{s}^2(g)
    &= g_{\mu\nu} \de{x}^\mu \otimes \de{x}^\nu \\
    &= \eta_{ab} \; \vi{a}{\mu}(x) \, \vi{b}{\nu}(x) \; \de{x}^\mu \otimes \de{x}^\nu \\
    &= \eta_{ab} \; \vif{a} \otimes \vif{b}.
  \end{split}
\end{equation}
Therefore, the vielbein, $\vif{a}$, is the fields equivalent to the metric tensor. In order to complete the structure, one needs information about the transport of geometrical objects lying on bundles based on $M$. That information is encoded on the spin connection, $\spif{a}{b}$. Using these quantities one finds  the generalisation of the structure equations of Cartan,
\begin{align}
  \df \vif{a} + \spif{a}{b} \we \vif{b} &= \Tf{a},
  \label{firstSE}\\
  \df \spif{a}{c} + \spif{a}{b} \we \spif{b}{c} &= \Rif{a}{c}
  \label{secondSE}.
\end{align}
In the sense of the previous lesson, the torsion 2-form, $\Tf{a}$, and the curvature 2-form,$\Rif{a}{c}$, measure the impossibility of endow an Euclidean structure on $M$.

\subsection*{Remarks on the Structure Equations}

\begin{itemize}
\item In general relativity, the torsion vanishes. Therefore, the first Cartan's structure Eq.~\eqref{firstSE}, yields an explicit expression for the spin connection as a function of the vielbein. This is equivalent to the well-known expression of the Levi-Civita connection $\Gamma_\mu{}^\lambda{}_\nu$ as a function of the metric and its derivatives.
\item The components of the torsion and curvature 2-forms are given by
%%%%
%% Change the eq. of the torsion (to be the equiv of the curvature
%%%%
  \begin{align}
    \Tf{a} &= \frac{1}{2} \tors{\mu}{a}{\nu} \; \de{x}^\mu \we \de{x}^\nu,
    \label{def-tor-comp} \\
    %\tor_\mu{}^\lambda{}_\nu \;\df\; x^\mu\w\df\; x^\nu &= \tor_a{}^c{}_b \vin{\lambda}{c}\;\vif{a}\w\vif{b},\\
    \Rif{a}{b} &= \frac{1}{2} \Ri^a{}_{b\mu\nu} \; \de{x}^\mu \we \de{x}^\nu.
    \label{def-curv-comp}
  \end{align}
\end{itemize}

\section{Playing with the Structure Equations}

From the first S.E.
\begin{align*}
  \df \( \df \vif{a} + \spif{a}{b} \we \vif{b} \) &= \df \Tf{a} \\
  \therefore \quad
  \df \Tf{a} &= \( \df \spif{a}{b}\) \we \vif{b} - \spif{a}{b} \we \df \vif{b}  \\
  \df \Tf{a} &= \( \Rif{a}{b} - \spif{a}{c} \we \spif{c}{b}\) \we \vif{b} - \spif{a}{c} \we \df \vif{c} \\
  \df \Tf{a} &= \Rif{a}{b} \we \vif{b} - \spif{a}{c} \we \( \spif{c}{b} \we \vif{b} + \df \vif{c} \) \\
  \df \Tf{a} &= \Rif{a}{b} \we \vif{b}-\spif{a}{c} \we \Tf{c},
  %  \Rif{a}{b} \we \vif{b}&=\cdf\Tf{a}
\end{align*}
then,
\begin{align}
  \Rif{a}{b} \we \vif{b}&=\df\Tf{a}+\spif{a}{c} \we \Tf{c}.
\end{align}


From the second S.E.
\begin{align*}
  \df\(\df\spif{a}{b}+\spif{a}{c} \we \spif{c}{b}\) &= \df\Rif{a}{b}\\
  \therefore \quad
  \df \Rif{a}{b} &= \(\df\spif{a}{c}\) \we \spif{c}{b}-\spif{a}{c} \we \(\df\spif{c}{b}\) \\
  \df \Rif{a}{b} &= \Rif{a}{c} \we \spif{c}{b}-\spif{a}{c} \we \Rif{c}{b},
\end{align*}
i.e.,
\begin{align}
  \df\Rif{a}{b} + \spif{a}{c} \we \Rif{c}{b} - \Rif{a}{c} \we \spif{c}{b}   &= 0.
\end{align}


\begin{WEbox}[%
    frametitle={Curvature of the 2-sphere},
    frametitlerule=true,
    frametitlealignment=\centering,
    frametitleaboveskip=10pt,]
  A 2-sphere  of radius $R$  has a line element given by
  \begin{align}
    \de{s}^2(g) = R^2 \( \de{\theta} \otimes \de{\theta} + \sin^2(\theta) \de{\phi} \otimes \de{\phi}\),
  \end{align}
  which can be written in terms of vielbeins as
  \begin{align}
    \de{s}^2(g) = \delta_{ij} \; \vif{i} \otimes \vif{j},
  \end{align}
  with 
  \begin{equation}
    \begin{split}
      \vif{1} &= R \de{\theta}, \\
      \vif{2} &= R \sin(\theta) \de{\phi}.
    \end{split}
  \end{equation}

  Using the first structure equation one gets,
  \begin{align}
    \df \vif{2}
    &=  R \cos(\theta) \de{\theta} \we \de{\phi} \notag \\
    &= -R \cos(\theta) \de{\phi} \we \de{\theta} \notag \\
    &= - \cos(\theta)  \de{\phi} \we \vif{1},
  \end{align}
  then
  \begin{align}
    \spif{2}{1} = \cos(\theta) \de{\phi}.
  \end{align}

  From the second structure equation, one obtains the only non-vanishing component of the 2-form curvature
  \begin{align}
    \Rif{2}{1} = -\Rif{1}{2} = \df \spif{2}{1} = - \sin(\theta) \de{\theta} \we \de{\phi}.
  \end{align}
  It follows from the last equation that
  \begin{align}
    \Rif{12}{} = \frac{1}{R^2}\vif{1} \we \vif{2},\label{curv-2sphere}
  \end{align}
  then, the 2-sphere is a manifold with constant curvature, as in Eq.~\eqref{def-const-curv}, with (Gau\ss{}ian) curvature $\kappa=\frac{1}{R^2}$.

  From Eqs.~\eqref{def-curv-comp} and~\eqref{curv-2sphere}, one obtains the non-vanishing component of the Riemann tensor,
  \begin{align}
    \Ri_{\theta\phi}{}^1{}_2 = \sin(\theta) \quad \Rightarrow \quad \Ri_{\theta\phi}{}^\theta{}_\phi = \sin^2(\theta).
  \end{align}
  Now, using the metric to raising and lowering indeces, and contracting, the Ricci and Ricci scalar are obtained,
  \begin{align}
    \Ri_{\theta\theta} & = 1, & & & \Ri_{\phi\phi} &= \sin^2(\theta), \\
    \intertext{and}
    & & \Ri &= \frac{2}{R^2} & & 
  \end{align}

  Finally, note that the 2-sphere is an Einstein manifold, since
  \begin{align}
    \Ri_{\mu\nu} = \frac{1}{R^2} g_{\mu\nu}.
  \end{align}
\end{WEbox}

\begin{WEbox}[%
    frametitle={Curvature of the 2-hyperboloid},
    frametitlerule=true,
    frametitlealignment=\centering,
    frametitleaboveskip=10pt,]
  The line element of a 2-hyperboloid is very similar to the one on the 2-sphere,
  \begin{align}
    \de{s}^2(g) = R^2 \( \de{\theta} \otimes \de{\theta} + \sinh^2(\theta) \de{\phi} \otimes \de{\phi} \),
  \end{align}
  then, the calculation of the curvature can be followed straightforward from the previous example. Thus, only the results are show,
  \begin{align}
    \vif{1} &= R \de{\theta} & \vif{2} &= R \sinh(\theta) \de{\phi} \\
    \spif{2}{1} &= \cosh(\theta) \de{\phi} & \Rif{2}{1} &= \sinh(\theta) \de{\theta} \we \de{\phi} \\
    \Ri_{\phi\theta}{}^2{}_1 &= - \sinh(\theta) & \Ri_{\phi\theta}{}^\phi{}_\theta &= -1 \\
    \Ri_{\theta\theta} &= -1 & \Ri_{\phi\phi} &= -\sinh^2(\theta).
  \end{align}
  The Ricci scalar is 
  \begin{align*}
    \Ri = -\frac{2}{R^2},
  \end{align*}
  and the hyperboloid is a manifold of constant curvature,
  \begin{align*}
    \Rif{12}{} = -\frac{1}{R^2} \vif{1} \we \vif{2},
  \end{align*}
  i.e., the Gau\ss{}ian curvature of the hyperboloid is $\kappa = -\frac{1}{R^2}$.
\end{WEbox}


\begin{WEbox}[%
    frametitle={Curvature of the four-dimensional $AdS$ spacetime},
    frametitlerule=true,
    frametitlealignment=\centering,
    frametitleaboveskip=10pt,]
  %% The curvature of the Anti de Sitter ($AdS$) spacetime is calculated, using Cartan's formalism.
  The metric of the $AdS_4$ spacetime is 
  \begin{align}
    \de{s}^2(g) = \frac{1}{z^2} \( -\de{t} \otimes \de{t} + \de{x} \otimes \de{x} + \de{y} \otimes \de{y} + \de{z} \otimes \de{z} \),
  \end{align}
  then the vielbeins are
  \begin{align}
    \vif{0} &= \frac{\de{t}}{z}, & \vif{1} &= \frac{\de{x}}{z}, \\
    \vif{2} &= \frac{\de{y}}{z}, & \vif{3} &= \frac{\de{z}}{z},
  \end{align}
  then,
  \begin{align}
    \df\vif{0} &= -\frac{1}{z^2} \de{z} \we \de{t} & \df\vif{1} &= -\frac{1}{z^2} \de{z} \we \de{x} \notag \\
    &= \frac{1}{z}\de{t} \we \vif{3} & &= \frac{1}{z}\de{x} \we \vif{3} \\
    \df\vif{2} &= -\frac{1}{z^2} \de{z} \we \de{y} & \df\vif{3} &=0 \notag  \\
    &= \frac{1}{z}\de{y} \we \vif{3} & & \notag
  \end{align}
  therefore,
  \begin{equation}
    \spif{0}{3} = -\frac{1}{z} \de{t}, \quad \spif{1}{3} = -\frac{1}{z} \de{x}, \quad \spif{2}{3} = -\frac{1}{z} \de{y}.
  \end{equation}
  Now, using the second structure equation, Eq.~\eqref{secondSE}, it follows that
  \begin{align}
    \Rif{0}{3} &= \df \spif{0}{3} = \frac{1}{z^2} \de{z} \we \de{t} &  \Rif{1}{3} &= \df \spif{1}{3} = \frac{1}{z^2} \de{z} \we \de{x} \notag \\
    \Rif{2}{3} &= \df \spif{2}{3} = \frac{1}{z^2} \de{z} \we \de{y} &  \Rif{0}{1} &= \spif{0}{3} \we \spif{3}{1} = -\frac{1}{z^2} \de{t} \we \de{x} \\
    \Rif{0}{2} &= \spif{0}{3} \we \spif{3}{2} = -\frac{1}{z^2}\de{t} \we \de{y} & \Rif{1}{2} &= \spif{1}{3} \we \spif{3}{2} = -\frac{1}{z^2}\de{x} \we \de{y}.\notag
  \end{align}
  
  Now, the non-vanishing components of the Riemann tensor are,
  \begin{align}
    \Ri^t{}_{ztz} &= -\frac{1}{z^2} & \Ri^x{}_{zxz} &= -\frac{1}{z^2}\notag\\
    \Ri^y{}_{zyz} &= -\frac{1}{z^2} & \Ri^t{}_{xtx} &= -\frac{1}{z^2}\\
    \Ri^t{}_{yty} &= -\frac{1}{z^2} & \Ri^x{}_{yxy} &= -\frac{1}{z^2}\notag\\
  \end{align}
  and finally, the Ricci tensor is
  \begin{align}
    \Ri_{\mu\nu} = -3 g_{\mu\nu}.
  \end{align}

  The $AdS$ spacetime is an example of an Einstein space, or in other words it is a solution of Einstein's equations with cosmological constant, $\Lambda=-3$.
\end{WEbox}

\begin{Ebox}
  Consider a Riemannian manifold with a metric whose line element is
  \begin{align}
    \de{s}^2(g) = -e^{2\Xi(r)} \de{t}\otimes \de{t} + e^{-2\Xi(r)} \de{r} \otimes\de{r} + r^2 \( \de{\theta} \otimes \de{\theta} + \sin^2(\theta) \de{\phi} \otimes \de{\phi} \).
  \end{align}
  Find the function $\Xi(r)$ which solves the Einstein's equation in the vacuum.
\end{Ebox}



\section[Hilbert-Einstein Action]{Hilbert-Einstein Action (\`a la Cartan)}



\begin{Pro}
  \begin{align*}
    S_{\text{gr}} = \frac{1}{2\kappa^2} \int \frac{\epsilon_{a_1\cdots a_D}}{(D-2)!} \Rif{a_1 a_2}{} \we \vif{a_3} \we \cdots \we \vif{a_D} = \frac{1}{2\kappa^2} \int \dn{D}{x} \abs{e} \Ri.
  \end{align*}
\end{Pro}
\begin{proof}
  \begin{align*}
    \frac{\epsilon_{a_1\cdots a_D}}{(D-2)!} \Rif{a_1 a_2}{} \we \vif{a_3} \we \cdots \we \vif{a_D}
    &=  \frac{\epsilon_{a_1\cdots a_D}}{(D-2)!} \frac{1}{2} \Ri^{a_1 a_2}{}_{cd} \; \vif{c} \we \vif{d} \we \vif{a_3} \we \cdots \we \vif{a_D} \\
    &= -\frac{\epsilon_{a_1\cdots a_D}}{(D-2)!} \frac{1}{2} \Ri^{a_1 a_2}{}_{cd} \; \epsilon^{c d a_3\cdots a_D} \de{V}\\
    &=  \frac{1}{2} \Ri^{a_1 a_2}{}_{cd} \( \delta_{a_1}^c \delta_{a_2}^d - \delta_{a_1}^d \delta_{a_2}^c \) \, \de{V}\\
    &=  \dn{D}{x} \abs{e} \Ri
  \end{align*}
\end{proof}

\section{Example of a non-Trivial Calculation}

Consider the metric whose line-element is
\begin{equation}
  \de{s}^2(g) = A^2 \[ - \frac{ (p^2 \de{\tau} + \de{\sigma})^2 }{ B^2 } + \frac{ (\de{\tau} - q^2 \de{\sigma})^2 }{ C^2 } + B^2 \de{q}^2 + C^2 \de{p}^2\],
\end{equation}
with $A$, $B$ and $C$ functions depending on $p$ and $q$.

Define,
\begin{align*}
  \bs{\tht}^0 &= p^2 \de{\tau} + \de{\sigma},\\
  \bs{\tht}^1 &= \de{\tau} - q^2 \de{\sigma}.
\end{align*}
Then,
\begin{align*}
  \de{\tau} &= \frac{ q^2 \bs{\tht}^0 + \bs{\tht}^1 }{ 1 + p^2 q^2 }, \\
  \de{\sigma} &= \frac{ \bs{\tht}^0 - p^2 \bs{\tht}^1 }{ 1 + p^2 q^2 }.
\end{align*}
Additionally,
\begin{align}
  \df[\bs{\tht}]^0
  &= \df \( p^2 \de{\tau} + \de{\sigma} \) \notag \\
  &= 2p \, \de{p}  \we \de{\tau} \notag \\
  &= \frac{ 2p }{ 1 + p^2 q^2 } \( q^2\, \de{p}  \we \bs{\tht}^0 + \de{p}  \we \bs{\tht}^1 \) \\
  \df[\bs{\tht}]^1
  &= \df \( \de{\tau} - q^2 \de{\sigma} \) \notag \\
  &= -2q \, \de{q}  \we \de{\sigma} \notag \\
  &= -\frac{ 2q }{ 1 + p^2 q^2 } \( \de{q}  \we \bs{\tht}^0 - p^2 \, \de{q}  \we \bs{\tht}^1 \).
\end{align}


Choosing the vielbeins by,
\begin{align}
  \vif{0} &= \frac{A}{B} \, \bs{\tht}^0,\\
  \vif{1} &= \frac{A}{C} \, \bs{\tht}^1,\\
  \vif{2} &= AB \, \de{q} ,\\
  \vif{3} &= AC \, \de{p} ,
\end{align}
their exterior derivative are
\begin{align}
  \df\vif{0} &= \partial_p \( \frac{A}{B} \) \, \de{p}  \we \bs{\tht}^0 + \partial_q \( \frac{A}{B} \) \, \de{q}  \we \bs{\tht}^0 + \frac{A}{B} \, \df[\bs{\tht}]^0, \\
  \df\vif{1} &= \partial_p \( \frac{A}{C} \) \, \de{p}  \we \bs{\tht}^1 + \partial_q \( \frac{A}{C} \) \, \de{q}  \we \bs{\tht}^1 + \frac{A}{C} \, \df[\bs{\tht}]^1, \\
  \df\vif{2} &= \partial_p(AB) \, \de{p}  \we \de{q}  , \\
  \df\vif{3} &= \partial_q(AC) \, \de{q}  \we \de{p} .
\end{align}

Now, 
\begin{equation}
  \begin{split}
    \df\vif{2}
    &= \partial_p(AB) \,\de{p}  \we \de{q} \\
    &= -\partial_p(AB) \,\de{q}  \we \de{p} \\
    &= -\frac{\partial_p(AB)}{AC} \,\de{q}  \we \vif{3} \\
    &= -\spif{2}{a} \we \vif{a},
  \end{split}
  \label{DLspi23}
\end{equation}
and
\begin{equation}
  \begin{split}
    \df\vif{3}
    &=  \partial_q(AC) \, \de{q}  \we \de{p}  \\
    &= -\partial_q(AC) \, \de{p}  \we \de{q}  \\
    &= -\frac{\partial_q(AC)}{AB} \, \de{p}  \we \vif{2} \\
    &= -\spif{3}{a} \we \vif{a}.
  \end{split}
  \label{DLspi32}
\end{equation}
Note that one needs to combine Eqs.~\eqref{DLspi23} and \eqref{DLspi32}, to obtain a consistent spin connection $\spif{23}{} = -\spif{32}{}$. The final result is therefore,
\begin{equation}
  \begin{split}
    \spif{2}{3}
    = \spif{23}{}
    = -\spif{32}{}
    =-\spif{3}{2}
    &= \frac{\partial_p(AB)}{AC} \,\de{q}  - \frac{\partial_q(AC)}{AB} \, \de{p}  \\
    &= \frac{1}{A^2BC} \[ \partial_p(AB) \, \vif{2} - {\partial_q(AC)} \, \vif{3} \].
  \end{split}
\end{equation}

From
\begin{equation}
  \begin{split}
    \df\vif{0}
    &= \partial_p \( \frac{A}{B} \) \, \de{p}  \we \bs{\tht}^0 + \partial_q \( \frac{A}{B} \) \, \de{q}  \we \bs{\tht}^0 + \frac{A}{B} \, \df[\bs{\tht}]^0 \\
    &= -\partial_p \( \frac{A}{B} \) \, \bs{\tht}^0 \we \de{p}  - \partial_q \( \frac{A}{B} \) \, \bs{\tht}^0 \we \de{q}  + \frac{ 2p }{ 1 + p^2 q^2 } \frac{A}{B} \( q^2 \, \de{p}  \we \bs{\tht}^0 + \de{p}  \we \bs{\tht}^1 \) \\
    %% &= -\frac{1}{AC}\partial_p\(\frac{A}{B}\)\, \bs{\tht}^0 \we \vif{3} - \frac{1}{AB}\partial_q\(\frac{A}{B}\)\, \bs{\tht}^0 \we \vif{2} + 2p\frac{A}{B}\,\frac{q^2\, \de{p}  \we \bs{\tht}^0 +\de{p}  \we \bs{\tht}^1}{1+p^2q^2}\notag\\
    %% &= -\frac{1}{A^2BC}\partial_p\(\frac{A}{B}\)\, \vif{0} \we \vif{3} - \frac{1}{A^2}\partial_q\(\frac{A}{B}\)\, \vif{0} \we \vif{2}\notag \\
    %% &{\phantom{=\;}} - 2p q^2\frac{A}{B}\,\frac{\bs{\tht}^0 \we \de{p}  }{1+p^2q^2}+ 2p\frac{A}{B}\,\frac{\de{p}  \we \bs{\tht}^1}{1+p^2q^2}\notag\\
    &= - \[ \frac{ B }{ A^2 C } \partial_p \( \frac{A}{B} \) + \frac{1}{AC} \, \frac{ 2 p q^2 }{ 1 + p^2 q^2 }  \] \, \vif{0} \we \vif{3} - \frac{1}{A^2} \partial_q \( \frac{A}{B} \) \, \vif{0} \we \vif{2} \\
    &\quad + \frac{ 2p }{ 1 + p^2 q^2 } \frac{1}{AB} \; \vif{3} \we \vif{1}\\
    &= -\spif{0}{a} \we \vif{a},
  \end{split}
\end{equation}
and,
\begin{equation}
  \begin{split}
    \df\vif{1}
    &= \partial_p \( \frac{A}{C} \) \, \de{p}  \we \bs{\tht}^1 + \partial_q \( \frac{A}{C} \) \, \de{q}  \we \bs{\tht}^1 + \frac{A}{C} \, \df[\bs{\tht}]^1 \\
    &= \partial_p \( \frac{A}{C} \) \, \de{p}  \we \bs{\tht}^1 + \partial_q \( \frac{A}{C} \) \, \de{q}  \we \bs{\tht}^1 - \frac{ 2q }{ 1 + p^2 q^2 } \frac{A}{C} \, \( \de{q}  \we \bs{\tht}^0 - p^2 \, \de{q}  \we \bs{\tht}^1 \) \\
    &= -\frac{1}{A^2} \partial_p \( \frac{A}{C} \) \, \vif{1} \we \vif{3} - \[ \frac{C}{A^2 B} \partial_q \( \frac{A}{C} \) + \frac{ 2 q p^2 }{ 1 + p^2 q^2 } \frac{1}{AB} \] \, \vif{1} \we \vif{2} \\
    &\quad - \frac{ 2q }{ 1 + p^2 q^2 } \frac{1}{AC} \, \vif{2} \we \vif{0} , \\
    &= -\spif{1}{a} \we \vif{a},
  \end{split}
\end{equation}
one obtains
\begin{align}
  \spif{0}{1} &= - \frac{ p }{ 1 + p^2 q^2 } \frac{1}{AB} \, \vif{3} + f_{01}, \\
  \spif{0}{2} &=   \frac{1}{A^2} \partial_q \( \frac{A}{B} \) \, \vif{0} - f_{02}, \\
  \spif{0}{3} &=  \[ \frac{B}{A^2 C} \partial_p \( \frac{A}{B} \) + \frac{ 2p q^2 }{ 1 + p^2 q^2 } \frac{1}{AC} \] \, \vif{0} + \frac{ p }{ 1 + p^2 q^2 } \frac{1}{AB} \, \vif{1} - f_{03}, \\
  \spif{1}{0} &= \frac{ q }{ 1 + p^2 q^2 } \frac{1}{AC} \, \vif{2} - f_{10}, \\
  \spif{1}{2} &= \[ \frac{ C }{ A^2 B } \partial_q \( \frac{A}{C} \) + \frac{ 2q p^2 }{ 1 + p^2 q^2 } \frac{1}{AB} \] \, \vif{1} - \frac{ q }{ 1 + p^2 q^2 }\frac{1}{AC} \, \vif{0} - f_{12}, \\
  \spif{1}{3} &= \frac{1}{A^2} \partial_p \( \frac{A}{C} \) \, \vif{1} - f_{13},
\end{align}
where the 1-forms $f_{ab}$ will be adjusted to get a consistent set of spin connection 1-forms.
